progs/verif_union.v
@@ -16,6 +16,7 @@ Definition fabs_single_spec :=
 Definition Gprog : funspecs :=
     ltac:(with_library prog [ fabs_single_spec ]).
 
+
 Lemma body_fabs_single: semax_body Vprog Gprog f_fabs_single fabs_single_spec.
 Proof.
 start_function.
@@ -40,9 +41,46 @@ Definition Gprog : funspecs :=
 
 Lemma body_fabs_single: semax_body Vprog Gprog f_fabs_single fabs_single_spec.
 Proof.
-start_function.
-assert_PROP(False).
-go_lower.
+try (start_function; fail 99).
 Abort.
 
 End Float.
+
+(*
+
+Lemma union_conversion:
+forall {CS} u sh p (i1 i2: ident) (t1 t2: type),
+  match PTree.get u (@cenv_cs CS) with
+  | Some {| co_su := Union; 
+            co_members := [(i1', t1'); (i2', t2')];
+            co_sizeof := 4;
+            co_rank := 0;
+         |}  => i1'=i1 /\ i2'=i2 /\ t1'=t1 /\ t2'=t2
+  | _ => False
+  end ->
+  i1 <> i2 ->
+  forall (x y: val) 
+        (v1 v2: reptype (nested_field_type (Tunion u noattr) [])),
+  JMeq v1 (@inl val val x) ->
+  JMeq v2 (@inr val val y) ->
+  (forall bl, 
+    Memdata.decode_val (chunk_of_type (typ_of_type t1)) bl = x <->
+    Memdata.decode_val (chunk_of_type (typ_of_type t2)) bl = y) ->
+  @field_at CS sh (Tunion u noattr) [] v1 p =
+  @field_at CS sh (Tunion u noattr) [] v2 p.
+Admitted.
+
+Lemma body_fabs_single: semax_body Vprog Gprog f_fabs_single fabs_single_spec.
+Proof.
+start_function.
+forward.
+clear.
+pose proof (union_conversion __125 Tsh v_u _f _i tfloat tuint).
+simpl in H.
+spec H; auto.
+spec H. compute; clear; congruence.
+evar (y: int).
+assert (reptype (Tunion __125 noattr) = (val+val)%type).
+reflexivity.
+
+*)
